template-coq/theories/WeakSubst.v
@@ -1,7 +1,7 @@
 (* Distributed under the terms of the MIT license.   *)
 
 From Coq Require Import Bool String List Program BinPos Compare_dec Omega.
-From Template Require Import config Ast Induction utils LiftSubst Typing.
+From Template Require Import config utils Ast AstUtils Induction utils LiftSubst Typing.
 
 (** * Weakening and substitution lemmas for typing derivations.
 
@@ -11,8 +11,8 @@ From Template Require Import config Ast Induction utils LiftSubst Typing.
 
 Set Asymmetric Patterns.
 
-Set Asymmetric Patterns.
 Generalizable Variables Σ Γ t T.
+Existing Instance default_checker_flags.
 
 Lemma length_app_context Γ Γ' : #|Γ ,,, Γ'| = #|Γ| + #|Γ'|.
 Proof.
@@ -36,7 +36,9 @@ Proof.
   unfold lift_context; induction Γ; simpl; trivial.
   simpl. destruct lift_context_rec. simpl in *.
   unfold lift_decl, map_decl. destruct a. simpl. rewrite IHΓ; f_equal.
-  rewrite lift_rec0. now destruct decl_body; simpl; rewrite ?lift_rec0.
+  f_equal.
+  now destruct decl_body; simpl; rewrite ?lift0_id.
+  now rewrite ?lift0_id.
 Qed.
 
 Lemma lift_context_rec_fst n k Γ :
@@ -155,30 +157,370 @@ Proof.
   - admit.
 Admitted.
 
-Inductive BoolSpecSet (P Q : Prop) : bool -> Set :=
-    BoolSpecT : P -> BoolSpecSet P Q true | BoolSpecF : Q -> BoolSpecSet P Q false.
+Require Import Lia.
 
-Lemma leb_spec_Set : forall x y : nat, BoolSpecSet (x <= y) (y < x) (x <=? y).
+Lemma lift_simpl (Γ'' Γ' : context) i t : i < #|Γ'| ->
+  lift0 (S i) (lift #|Γ''| (#|Γ'| - S i) t) = lift #|Γ''| #|Γ'| (lift0 (S i) t).
 Proof.
-  intros.
-  destruct (Nat.leb_spec0 x y).
-  now constructor.
-  constructor. now auto with arith.
+  intros. assert (#|Γ'| = S i + (#|Γ'| - S i)) by easy.
+  rewrite H0 at 2.
+  rewrite <- permute_lift; try easy.
 Qed.
 
+Lemma nth_map {A} (f : A -> A) n l d :
+  (d = f d) ->
+  nth n (map f l) d = f (nth n l d).
+Proof.
+  induction n in l |- *; destruct l; simpl; auto.
+Qed.
+
+Lemma lift_iota_red n k pars c args brs :
+  lift n k (iota_red pars c args brs) =
+  iota_red pars c (List.map (lift n k) args) (List.map (on_snd (lift n k)) brs).
+Proof.
+  unfold iota_red. rewrite !lift_mkApps. f_equal; auto using map_skipn.
+  rewrite nth_map; simpl; auto.
+Qed.
+
+Definition lift_subst n k s :=
+  List.fold_right (fun t l => lift n (List.length l + k) t :: l) [] s.
+
+Lemma lift_subst_length n k s : #|lift_subst n k s| = #|s|.
+Proof.
+  induction s in n, k |- *; simpl; auto.
+Qed.
+
+Lemma fix_subst_length mfix : #|fix_subst mfix| = #|mfix|.
+Proof.
+  unfold fix_subst. generalize (tFix mfix). intros.
+  induction mfix; simpl; auto.
+Qed.
+
+Lemma cofix_subst_length mfix : #|cofix_subst mfix| = #|mfix|.
+Proof.
+  unfold cofix_subst. generalize (tCoFix mfix). intros.
+  induction mfix; simpl; auto.
+Qed.
+
+Require Import Compare_dec Lia.
+
+Lemma parsubst_empty k a : Ast.wf a -> parsubst [] k a = a.
+Proof.
+  induction 1 in k |- * using term_wf_forall_list_ind; simpl; try congruence;
+    try solve [f_equal; eauto; apply_spec; eauto].
+
+  - elim (Nat.compare_spec k n); destruct (Nat.leb_spec k n); intros; try easy.
+    subst. rewrite Nat.sub_diag. simpl. rewrite Nat.sub_0_r. reflexivity.
+    assert (n - k > 0) by lia.
+    assert (exists n', n - k = S n'). exists (pred (n - k)). lia.
+    destruct H2. rewrite H2. simpl. now rewrite Nat.sub_0_r.
+  - rewrite IHwf. rewrite mkApps_tApp; eauto with wf.
+    f_equal; apply_spec. auto.
+  - rewrite IHwf, IHwf0. f_equal. red in H. apply_spec. intros; eauto.
+    destruct x; unfold on_snd; simpl in *; congruence.
+  - f_equal. clear H0. red in H; apply_spec. intuition auto.
+    destruct x; unfold map_def; simpl in *; congruence.
+  - f_equal. red in H; apply_spec. intuition auto.
+    destruct x; unfold map_def; simpl in *; congruence.
+Qed.
+
+Lemma lift_unfold_fix n k mfix idx narg fn :
+  unfold_fix mfix idx = Some (narg, fn) ->
+  unfold_fix (map (map_def (lift n k) (lift n (#|mfix| + k))) mfix) idx = Some (narg, lift n k fn).
+Proof.
+  unfold unfold_fix.
+  rewrite nth_error_map. destruct (nth_error mfix idx) eqn:Hdef; try congruence.
+  intros [= <- <-]. simpl. repeat f_equal. unfold substl.
+  rewrite (distr_lift_subst_rec _ _ n 0 k).
+  rewrite fix_subst_length. f_equal.
+  unfold fix_subst. rewrite !map_length.
+  generalize #|mfix| at 2 3. induction n0; auto. simpl.
+  f_equal. apply IHn0.
+Qed.
+Hint Resolve lift_unfold_fix.
+
+Lemma lift_unfold_cofix n k mfix idx narg fn :
+  unfold_cofix mfix idx = Some (narg, fn) ->
+  unfold_cofix (map (map_def (lift n k) (lift n (#|mfix| + k))) mfix) idx = Some (narg, lift n k fn).
+Proof.
+  unfold unfold_cofix.
+  rewrite nth_error_map. destruct (nth_error mfix idx) eqn:Hdef; try congruence.
+  intros [= <- <-]. simpl. repeat f_equal. unfold substl.
+  rewrite (distr_lift_subst_rec _ _ n 0 k).
+  rewrite cofix_subst_length. f_equal.
+  unfold cofix_subst. rewrite !map_length.
+  generalize #|mfix| at 2 3. induction n0; auto. simpl.
+  f_equal. apply IHn0.
+Qed.
+Hint Resolve lift_unfold_cofix.
+
+Lemma lift_is_constructor:
+  forall (args : list term) (narg : nat) n k,
+    is_constructor narg args = true -> is_constructor narg (map (lift n k) args) = true.
+Proof.
+  intros args narg.
+  unfold is_constructor; intros.
+  rewrite nth_error_map. destruct nth_error; try discriminate. simpl. intros.
+  destruct t; try discriminate || reflexivity.
+  destruct t; try discriminate || reflexivity.
+Qed.
+Hint Resolve lift_is_constructor.
+
+Hint Rewrite UnivSubst.lift_subst_instance_constr : lift.
+Hint Rewrite lift_mkApps : lift.
+Hint Rewrite distr_lift_subst : lift.
+Hint Rewrite lift_iota_red : lift.
+
+Definition map_constant_body f decl :=
+  {| cst_type := f decl.(cst_type);
+     cst_body := option_map f decl.(cst_body);
+     cst_universes := decl.(cst_universes) |}.
+
+Lemma map_cst_type f decl : f (cst_type decl) = cst_type (map_constant_body f decl).
+Proof. destruct decl; reflexivity. Qed.
+
+Lemma map_cst_body f decl : option_map f (cst_body decl) = cst_body (map_constant_body f decl).
+Proof. destruct decl; reflexivity. Qed.
+
+Lemma map_dtype {A B : Set} (f : A -> B) (g : A -> B) (d : def A) :
+  f (dtype d) = dtype (map_def f g d).
+Proof. destruct d; reflexivity. Qed.
+
+Lemma map_dbody {A B : Set} (f : A -> B) (g : A -> B) (d : def A) :
+  g (dbody d) = dbody (map_def f g d).
+Proof. destruct d; reflexivity. Qed.
+
+Lemma declared_decl_info `{checker_flags} Σ c decl :
+  type_global_env (snd Σ) (fst Σ) ->
+  lookup_env (fst Σ) c = Some decl ->
+  { Σ' & { wfΣ' : type_global_env (snd Σ) Σ' & type_global_decl (Σ', snd Σ) decl } }.
+Proof.
+  induction 1; simpl. congruence.
+  destruct ident_eq. intros [= ->].
+  exists Σ0. exists X. auto.
+  apply IHX.
+Qed.
+
+Lemma lift_declared_constant `{checker_flags} Σ cst decl n k :
+  wf Σ ->
+  declared_constant (fst Σ) cst decl ->
+  decl = map_constant_body (lift n k) decl.
+Proof.
+  unfold declared_constant.
+  intros.
+  eapply declared_decl_info in H0; auto.
+  destruct H0 as [Σ' [wfΣ' decl']].
+  red in decl'. red in decl'.
+  destruct decl. simpl in *. destruct cst_body. unfold map_constant_body. simpl.
+  pose proof decl' as declty.
+  apply typecheck_closed in declty; eauto.
+  destruct declty as [declty Hcl].
+  rewrite andb_true_iff in Hcl. destruct Hcl as [clb clty].
+  pose proof (closed_upwards _ _ clb k).
+  pose proof (closed_upwards _ _ clty k).
+  simpl in *. forward H0 by lia. forward H1 by lia.
+  apply (lift_closed n k) in H0.
+  apply (lift_closed n k) in H1. rewrite H0, H1. reflexivity.
+  constructor.
+  red in decl'.
+  destruct decl'.
+  apply typecheck_closed in t. destruct t as [_ ccst].
+  rewrite andb_true_iff in ccst. destruct ccst as [ccst _].
+  eapply closed_upwards in ccst; simpl.
+  apply (lift_closed n k) in ccst. unfold map_constant_body. simpl.
+  rewrite ccst. reflexivity. lia. auto. constructor.
+Qed.
+
+(* Lemma forall_decls_declared_minductive Σ cst decl : *)
+(*   declared_minductive Σ cst decl -> *)
+(*   declared_minductive (trans_global_decls Σ) cst (trans_minductive_body decl). *)
+(* Proof. *)
+(*   unfold declared_minductive, TTy.declared_minductive. *)
+(*   induction Σ => //; try discriminate. *)
+(*   case: a => // /= k b; case: (ident_eq cst k); auto. *)
+(*   - by discriminate. *)
+(*   - by move => [=] -> ->. *)
+(* Qed. *)
+
+(* Lemma forall_decls_declared_inductive Σ cst univs decl : *)
+(*   TTy.declared_inductive Σ cst univs decl -> *)
+(*   declared_inductive (trans_global_decls Σ) cst univs (trans_one_ind_body decl). *)
+(* Proof. *)
+(*   unfold declared_inductive, TTy.declared_inductive. *)
+(*   move=> [decl' [H [Hu Hnth]]]. *)
+(*   pose proof (forall_decls_declared_minductive _ _ _ H). *)
+(*   eexists. split; eauto. destruct decl'; simpl in *. *)
+(*   subst univs. split; auto. *)
+(*   by rewrite nth_error_map Hnth. *)
+(* Qed. *)
+
+Lemma weakening_red1 `{CF:checker_flags} Σ Γ Γ' Γ'' M N :
+  type_global_env (snd Σ) (fst Σ) ->
+  red1 (fst Σ) (Γ ,,, Γ') M N ->
+  red1 (fst Σ) (Γ ,,, Γ'' ,,, lift_context #|Γ''| 0 Γ') (lift #|Γ''| #|Γ'| M) (lift #|Γ''| #|Γ'| N).
+Proof.
+  intros wfΣ H.
+  remember (Γ ,,, Γ') as Γ0. revert Γ Γ' Γ'' HeqΓ0.
+  induction H using red1_ind_all in |- *; intros Γ0 Γ' Γ'' HeqΓ0; try subst Γ; simpl;
+    autorewrite with lift;
+    try solve [  econstructor; eauto ].
+
+  - elim (leb_spec_Set); intros Hn.
+    + rewrite simpl_lift; try lia. rewrite Nat.add_succ_r.
+      destruct (weaken_safe_nth_ge _ _ _ isdecl Γ'' Hn) as [isdecl' Heq].
+      rewrite Heq in H.
+      unshelve econstructor; eauto.
+    + destruct (weaken_safe_nth_lt _ _ _ isdecl Γ'' Hn) as [isdecl' Heq].
+      rewrite <- lift_simpl by easy.
+      econstructor.
+      apply (f_equal decl_body) in Heq.
+      rewrite Heq. unfold lift_decl. simpl. now rewrite H.
+
+  - econstructor.
+    eauto. rewrite H0. f_equal.
+    eapply (declared_decl_info _ _ _ wfΣ) in H.
+    destruct H as [Σ' [wfΣ' decl']].
+    red in decl'. red in decl'.
+    rewrite H0 in decl'.
+    apply typecheck_closed in decl'; eauto. destruct decl'.
+    rewrite andb_true_iff in e. destruct e as [Hclosed _].
+    simpl in Hclosed.
+    pose proof (closed_upwards _ _ Hclosed #|Γ'|).
+    forward H by lia.
+    apply (lift_closed #|Γ''| #|Γ'|) in H. auto.
+    constructor.
+
+  - simpl. rewrite <- nth_map by reflexivity.
+    constructor.
+
+  - constructor.
+    specialize (IHred1 Γ0 (Γ' ,, vass na N) Γ'' eq_refl).
+    rewrite lift_context_snoc, Nat.add_0_r in IHred1. apply IHred1.
+
+  - constructor.
+    specialize (IHred1 Γ0 (Γ' ,, vdef na b t) Γ'' eq_refl).
+    rewrite lift_context_snoc, Nat.add_0_r in IHred1. apply IHred1.
+
+  - constructor.
+    induction H; constructor; auto.
+    intuition; eauto.
+    apply H0. auto.
+
+  - constructor.
+    induction H; constructor; auto.
+    intuition; eauto.
+
+  - constructor.
+    specialize (IHred1 Γ0 (Γ' ,, vass na M1) Γ'' eq_refl).
+    rewrite lift_context_snoc, Nat.add_0_r in IHred1. apply IHred1.
+
+  - constructor.
+    induction H; constructor; auto.
+    intuition; eauto.
+Qed.
+
+Lemma lift_eq_term `{checker_flags} ϕ n k T U :
+  eq_term ϕ T U = true ->
+  eq_term ϕ (lift n k T) (lift n k U) = true.
+Proof.
+  intros Hleq.
+  induction T in n, k, U, Hleq |- * using term_forall_list_ind; intros;
+    destruct U; try discriminate;
+  try solve [simpl; auto]; try
+                             (destruct (mkApps_trans_wf _ _ H0) as [U' [V' ->]]; reflexivity);
+  simpl in *; revert Hleq; try rewrite !andb_true_iff in *; intuition auto;
+    try (merge_Forall; close_Forall; intuition auto).
+
+  - intros. apply Nat.eqb_eq in Hleq. subst.
+    destruct Nat.leb; simpl. apply Nat.eqb_eq. reflexivity. apply Nat.eqb_refl.
+  - destruct p. destruct Nat.leb. discriminate. discriminate.
+  - destruct p, p0. rewrite !andb_true_iff in *. intuition auto.
+    red in H0. merge_Forall. close_Forall. intuition auto. destruct y. simpl. auto.
+  - rewrite !andb_true_iff in *.
+    destruct x, y; simpl in *; intuition auto.
+    assert (#|m| = #|m0|). clear -H2. induction H2; simpl; auto. rewrite H4. auto.
+  - rewrite !andb_true_iff in *.
+    destruct x, y; simpl in *; intuition auto.
+    assert (#|m| = #|m0|). clear -H2. induction H2; simpl; auto. rewrite H4. auto.
+Qed.
+
+Lemma lift_leq_term `{checker_flags} ϕ n k T U :
+  leq_term ϕ T U = true ->
+  leq_term ϕ (lift n k T) (lift n k U) = true.
+Proof.
+  intros Hleq.
+  induction T in n, k, U, Hleq |- * using term_forall_list_ind; intros;
+    destruct U; try discriminate;
+  try solve [simpl; auto]; try
+                             (destruct (mkApps_trans_wf _ _ H0) as [U' [V' ->]]; reflexivity);
+  simpl in *; revert Hleq; try destruct p, p0; try rewrite !andb_true_iff in *;
+    intuition auto using lift_eq_term;
+    try (merge_Forall; close_Forall; intuition eauto using lift_eq_term).
+
+  - intros. apply Nat.eqb_eq in Hleq. subst.
+    destruct Nat.leb; simpl. apply Nat.eqb_eq. reflexivity. apply Nat.eqb_refl.
+  - destruct p. destruct (Nat.leb k n0); discriminate.
+  - destruct y. simpl. auto using lift_eq_term.
+  - rewrite !andb_true_iff in *.
+    destruct x, y; simpl in *; intuition auto using lift_eq_term.
+    assert (#|m| = #|m0|). clear -H2. induction H2; simpl; auto. rewrite H4.
+    auto using lift_eq_term.
+  - rewrite !andb_true_iff in *.
+    destruct x, y; simpl in *; intuition auto using lift_eq_term.
+    assert (#|m| = #|m0|). clear -H2. induction H2; simpl; auto. rewrite H4.
+    auto using lift_eq_term.
+Qed.
+
+Lemma weakening_cumul `{CF:checker_flags} Σ Γ Γ' Γ'' M N :
+  type_global_env (snd Σ) (fst Σ) ->
+  Σ ;;; Γ ,,, Γ' |- M <= N ->
+  Σ ;;; Γ ,,, Γ'' ,,, lift_context #|Γ''| 0 Γ' |- lift #|Γ''| #|Γ'| M <= lift #|Γ''| #|Γ'| N.
+Proof.
+  intros wfΣ. induction 1.
+  constructor.
+  - now apply lift_leq_term.
+  - eapply weakening_red1 in H; auto.
+    econstructor 2; eauto.
+  - eapply weakening_red1 in H0; auto.
+    econstructor 3; eauto.
+Qed.
+
+Lemma nlt_map {A B} (l : list A) (f : A -> B) (n : {n | n < #|l| }) : `n < #|map f l|.
+Proof. destruct n. simpl. now rewrite map_length. Defined.
+
+Lemma map_def_safe_nth {A B} (l : list A) (n : {n | n < #|l| }) (f : A -> B) :
+  f (safe_nth l n) = safe_nth (map f l) (exist _ (`n) (nlt_map l f n)).
+Proof.
+  destruct n.
+  induction l in x, l0 |- *. simpl. bang.
+  simpl. destruct x. reflexivity. simpl.
+  rewrite IHl. f_equal. f_equal. pi.
+Qed.
+
+Lemma wf_local_app `{checker_flags} Σ (Γ Γ' : context) : wf_local Σ (Γ ,,, Γ') -> wf_local Σ Γ.
+Admitted.
+
 Lemma weakening_rec `{cf : checker_flags} Σ Γ Γ' Γ'' (t : term) :
-  type_global_env (snd Σ) (fst Σ) -> wf_local Σ (Γ ,,, Γ') ->
+  type_global_env (snd Σ) (fst Σ) ->
+  wf_local Σ (Γ ,,, Γ') -> (* Not necessary now *)
   wf_local Σ (Γ ,,, Γ'' ,,, lift_context #|Γ''| 0 Γ') ->
   `(Σ ;;; Γ ,,, Γ' |- t : T ->
     Σ ;;; Γ ,,, Γ'' ,,, lift_context #|Γ''| 0 Γ' |-
     lift #|Γ''| #|Γ'| t : lift #|Γ''| #|Γ'| T).
 Proof.
-  intros HΣ HΓΓ' HΓ'' * H. revert Γ'' HΓ''.
-  dependent induction H; intros Γ'' HΓ''; simpl in *; try solve [econstructor; eauto].
+  intros HΣ HΓΓ' HΓ'' * H.
+  generalize_eqs H. intros eqw. rewrite <- eqw in HΓΓ'.
+  revert Γ Γ' Γ'' HΓ'' eqw.
+  revert Σ HΣ Γ0 HΓΓ' t T H.
+  apply (typing_ind_env (fun Σ Γ0 t T =>  forall Γ Γ' Γ'' : context,
+    wf_local Σ (Γ ,,, Γ'' ,,, lift_context #|Γ''| 0 Γ') ->
+    Γ0 = Γ ,,, Γ' ->
+    Σ;;; Γ ,,, Γ'' ,,, lift_context #|Γ''| 0 Γ' |- lift #|Γ''| #|Γ'| t : lift #|Γ''| #|Γ'| T));
+    intros Σ wfΣ Γ0 wfΓ0; intros; subst Γ0; simpl in *; try solve [econstructor; eauto].
 
   - elim (leb_spec_Set); intros Hn.
     + destruct (weaken_safe_nth_ge _ _ _ isdecl Γ'' Hn) as [isdecl' ->].
-      rewrite simpl_lift_rec; try omega. rewrite Nat.add_succ_r.
+      rewrite simpl_lift; try omega. rewrite Nat.add_succ_r.
       constructor. auto.
     + destruct (weaken_safe_nth_lt _ _ _ isdecl Γ'' Hn) as [isdecl' H'].
       apply (f_equal decl_type) in H'.
@@ -186,64 +528,95 @@ Proof.
       assert (forall t, lift0 (S n) (lift #|Γ''| (#|Γ'| - S n) t) = lift #|Γ''| #|Γ'| (lift0 (S n) t)).
       intros. assert (#|Γ'| = S n + (#|Γ'| - S n)) by easy.
       rewrite H at 2.
-      rewrite <- permute_lift_rec; try easy.
+      rewrite <- permute_lift; try easy.
       rewrite <- H. rewrite <- H'. constructor. auto.
 
   - econstructor; auto.
-    simpl.
-    specialize (IHtyping2 Γ (Γ' ,, vass n t) HΣ).
-    forward IHtyping2. econstructor; eauto.
-    specialize (IHtyping2 eq_refl Γ'').
-    forward IHtyping2. rewrite lift_context_snoc. econstructor; eauto.
-    simpl. rewrite Nat.add_0_r. eapply IHtyping1; auto.
-    rewrite lift_context_snoc, plus_0_r in IHtyping2.
-    eapply IHtyping2.
+    specialize (X2 Γ (Γ' ,, vass n t) Γ'').
+    forward X2. rewrite lift_context_snoc. simpl. econstructor; eauto.
+    simpl. rewrite Nat.add_0_r. eapply X0; auto.
+    rewrite lift_context_snoc, plus_0_r in X2.
+    eapply X2. reflexivity.
 
   - econstructor; auto.
     simpl.
-    specialize (IHtyping2 Γ (Γ' ,, vass n t) HΣ).
-    forward IHtyping2. econstructor; eauto.
-    specialize (IHtyping2 eq_refl Γ'').
-    forward IHtyping2. rewrite lift_context_snoc. econstructor; eauto.
-    rewrite Nat.add_0_r. eapply IHtyping1; auto.
-    rewrite lift_context_snoc, plus_0_r in IHtyping2.
-    eapply IHtyping2.
+    specialize (X2 Γ (Γ' ,, vass n t) Γ'').
+    forward X2. rewrite lift_context_snoc. simpl; econstructor; eauto.
+    simpl.  rewrite Nat.add_0_r. eapply X0; auto.
+    rewrite lift_context_snoc, plus_0_r in X2.
+    eapply X2. reflexivity.
 
   - econstructor; auto.
-    simpl.
-    specialize (IHtyping3 Γ (Γ' ,, vdef n b b_ty) HΣ).
-    forward IHtyping3. constructor; simpl; auto.
-    specialize (IHtyping3 eq_refl Γ'').
-    forward IHtyping3. rewrite lift_context_snoc, Nat.add_0_r.
-    simpl.
-    constructor. simpl; auto.
-    simpl. eapply IHtyping2; auto. simpl.
-    rewrite lift_context_snoc, plus_0_r in IHtyping3.
-    eapply IHtyping3.
+    specialize (X2 Γ Γ' Γ'' X5 eq_refl). simpl.
+    specialize (X4 Γ (Γ' ,, vdef n b b_ty) Γ'').
+    forward X4. rewrite lift_context_snoc. simpl; econstructor; eauto.
+    simpl. rewrite Nat.add_0_r. auto.
+    rewrite lift_context_snoc, plus_0_r in X4. apply X4. reflexivity.
 
   - econstructor; auto.
-    now apply lift_rec_isApp.
+    now apply lift_isApp.
     now apply map_non_nil.
+    clear X0 X H0 H.
+    induction X1. econstructor; eauto.
+    eapply type_spine_cons.
+    simpl in p. apply p; auto.
+    change (tProd na (lift #|Γ''| #|Γ'| A) (lift #|Γ''| (S #|Γ'|) B))
+      with (lift #|Γ''| #|Γ'| (tProd na A B)).
+    eapply weakening_cumul; eauto. auto.
+    rewrite distr_lift_subst in IHX1. apply IHX1.
+
+  - autorewrite with lift.
+    rewrite map_cst_type. constructor.
+    erewrite <- lift_declared_constant; eauto.
+    erewrite <- lift_declared_constant; eauto.
+
+  - autorewrite with lift.
     admit.
 
   - admit.
-  - admit.
-  - admit.
 
-  - admit.
-  - admit.
-  - admit.
-  - (* Conv *)
+  - rewrite map_app, map_skipn.
+    specialize (X3 _ _ _ X5 eq_refl).
+    specialize (X1 _ _ _ X5 eq_refl).
+    specialize (X0 _ _ _ X5 eq_refl).
+    simpl. econstructor; eauto 2.
+    admit. admit.
+
+    rewrite lift_mkApps in X3. eauto.
+    eapply (Forall2_map _ _ (on_snd (lift #|Γ''| #|Γ'|)) brs btys). close_Forall.
+    intros.
+    intuition. destruct x, y; simpl in *. subst n0.
+    apply b; auto.
+
+  - unfold substl. simpl.
+    erewrite (distr_lift_subst_rec _ _ _ 0 #|Γ'|).
+    simpl. rewrite map_rev.
+    subst ty.
+    rewrite List.rev_length.
+    replace (lift #|Γ''| (S (#|args| + #|Γ'|)) (snd decl))
+      with (snd (on_snd (lift #|Γ''| (S (#|args| + #|Γ'|))) decl)) by now destruct decl.
+    econstructor. admit.
+    specialize (X0 _ _ _ X1 eq_refl).
+    rewrite lift_mkApps in X0. eapply X0.
+
+  - subst ty.
+    erewrite map_dtype, map_def_safe_nth. simpl.
+    eapply type_Fix. admit.
     admit.
+
+  - subst ty.
+    erewrite map_dtype, map_def_safe_nth. simpl.
+    eapply type_CoFix. admit.
+    admit.
+
+  - econstructor; eauto.
+    now eapply weakening_cumul.
 Admitted.
 
-Lemma wf_local_app `{checker_flags} Σ (Γ Γ' : context) : wf_local Σ (Γ ,,, Γ') -> wf_local Σ Γ.
-Admitted.
-
-Lemma weakening `{cf : checker_flags} Σ Γ Γ' (t : term) :
+Lemma weakening `{cf : checker_flags} Σ Γ Γ' (t : term) T :
   type_global_env (snd Σ) (fst Σ) -> wf_local Σ (Γ ,,, Γ') ->
-  `(Σ ;;; Γ |- t : T ->
-    Σ ;;; Γ ,,, Γ' |- lift0 #|Γ'| t : lift0 #|Γ'| T).
+  Σ ;;; Γ |- t : T ->
+  Σ ;;; Γ ,,, Γ' |- lift0 #|Γ'| t : lift0 #|Γ'| T.
 Proof.
   intros HΣ HΓΓ' * H.
   pose (weakening_rec Σ Γ [] Γ' t).
@@ -251,7 +624,22 @@ Proof.
   forward t0; eauto. now eapply wf_local_app in HΓΓ'.
 Qed.
 
-Lemma substitution `{checker_flags} Σ Γ n u U (t : term) :
+Inductive subs Σ (Γ : context) : list term -> context -> Type :=
+| emptys : subs Σ Γ [] []
+| conss Δ s na t T : subs Σ Γ s Δ ->
+              Σ ;;; Γ |- t : substl s T ->
+              subs Σ Γ (t :: s) (Δ ,, vass na T).
+
+Theorem substitution `{checker_flags} Σ Γ Γ' s Δ (t : term) T :
+  type_global_env (snd Σ) (fst Σ) -> wf_local Σ Γ ->
+  subs Σ Γ s Γ' ->
+  Σ ;;; Γ ,,, Γ' ,,, Δ |- t : T ->
+  Σ ;;; Γ ,,, map_context (substl s) Δ |- substl s t : substl s T.
+Proof.
+  intros HΣ HΓ * Ht Hu.
+Admitted.
+
+Lemma substitution0 `{checker_flags} Σ Γ n u U (t : term) :
   type_global_env (snd Σ) (fst Σ) -> wf_local Σ Γ ->
   `(Σ ;;; Γ ,, vass n U |- t : T -> Σ ;;; Γ |- u : U ->
     Σ ;;; Γ |- t {0 := u} : T {0 := u}).
