template-coq/theories/Induction.v
@@ -35,8 +35,8 @@ Lemma term_forall_list_ind :
         P t -> forall t0 : term, P t0 -> forall l : list (nat * term),
             tCaseBrsProp P l -> P (tCase p t t0 l)) ->
     (forall (s : projection) (t : term), P t -> P (tProj s t)) ->
-    (forall (m : mfixpoint term) (n : nat), tFixProp P m -> P (tFix m n)) ->
-    (forall (m : mfixpoint term) (n : nat), tFixProp P m -> P (tCoFix m n)) ->
+    (forall (m : mfixpoint term) (n : nat), tFixProp P P m -> P (tFix m n)) ->
+    (forall (m : mfixpoint term) (n : nat), tFixProp P P m -> P (tCoFix m n)) ->
     forall t : term, P t.
 Proof.
   intros until t. revert t.
@@ -107,8 +107,8 @@ Lemma term_wf_forall_list_ind :
         P t -> forall t0 : term, P t0 -> forall l : list (nat * term),
             tCaseBrsProp P l -> P (tCase p t t0 l)) ->
     (forall (s : projection) (t : term), P t -> P (tProj s t)) ->
-    (forall (m : mfixpoint term) (n : nat), tFixProp P m -> Forall (fun def => isLambda (dbody def) = true) m -> P (tFix m n)) ->
-    (forall (m : mfixpoint term) (n : nat), tFixProp P m -> P (tCoFix m n)) ->
+    (forall (m : mfixpoint term) (n : nat), tFixProp P P m -> Forall (fun def => isLambda (dbody def) = true) m -> P (tFix m n)) ->
+    (forall (m : mfixpoint term) (n : nat), tFixProp P P m -> P (tCoFix m n)) ->
     forall t : term, wf t -> P t.
 Proof.
   intros until t. revert t.
